Mica/Verifier.lean
@@ -6,6 +6,7 @@ import Mica.Verifier.Bindings
 import Mica.Verifier.Utils
 import Mica.Verifier.Assertions
 import Mica.Verifier.Intrinsic
+import Mica.Verifier.BoundedQuantifier
 import Mica.Verifier.Expressions
 import Mica.Verifier.RelationalEncoding
 import Mica.Verifier.Functions
